Start proving the Stenning example

fairneris/examples/stenning_code.v
@@ -1,10 +1,20 @@
-From fairneris.aneris_lang Require Export lang.
+From stdpp Require Import list fin_maps.
+From iris.algebra Require Import excl_auth.
+From iris.proofmode Require Import proofmode.
+From iris.base_logic.lib Require Import invariants.
+From trillium.program_logic Require Import ectx_lifting.
+From fairneris Require Import fairness fair_resources fuel.
+From fairneris.examples Require Import stenning_model.
+From fairneris.aneris_lang Require Import proofmode.
+From fairneris.aneris_lang.state_interp Require Import state_interp state_interp_events.
+From fairneris.aneris_lang.program_logic Require Import aneris_weakestpre.
 
 Definition client (sa_clt sa_srv : socket_address) : val :=
   λ: <>,
      let: "sh_clt" := NewSocket #() in
      SocketBind "sh_clt" #sa_clt;;
-     (rec: "f" "i" :=
+     SetReceiveTimeout "sh_clt" #1 #1;;
+     let: "go" := (rec: "f" "i" :=
         SendTo "sh_clt" "sa_srv" (i2s "i");;
         match: (ReceiveFrom "sh_clt") with
           NONE     => "f" "i"
@@ -16,13 +26,15 @@ Definition client (sa_clt sa_srv : socket_address) : val :=
                         else "f" "i"
                       else
                         "f" "i"
-        end) #0.
+        end)
+     in "go" #0.
 
 Definition server (sa_clt sa_srv : socket_address) : val :=
   λ: <>,
      let: "sh_srv" := NewSocket #() in
      SocketBind "sh_srv" #sa_srv;;
-     (rec: "f" "j" :=
+     SetReceiveTimeout "sh_srv" #1 #1;;
+     let: "go" := (rec: "f" "j" :=
         match: (ReceiveFrom "sh_srv") with
           NONE     => "f" "j"
         | SOME "m" => if: Snd "m" = "sa_clt"
@@ -33,4 +45,109 @@ Definition server (sa_clt sa_srv : socket_address) : val :=
                         else SendTo "sh_srv" "sa_clt" "j";; "f" "j"
                       else
                         "f" "j"
-        end) #-1.
+        end)
+     in "go" #-1.
+
+Canonical Structure stenning_A_stateO := leibnizO stenning_A_state.
+Canonical Structure stenning_B_stateO := leibnizO stenning_B_state.
+
+Class stenningG Σ := StenningG {
+  stenning_A_name: gname;
+  stenning_B_name: gname;
+  stenning_A_G :> inG Σ (excl_authR stenning_A_stateO);
+  stenning_B_G :> inG Σ (excl_authR stenning_B_stateO);
+ }.
+Class stenningPreG Σ := {
+  stenning_A_PreG :> inG Σ (excl_authR stenning_A_stateO);
+  stenning_B_PreG :> inG Σ (excl_authR stenning_B_stateO);
+ }.
+Definition stenningΣ : gFunctors :=
+  #[ anerisΣ (live_model_of_user stenning_model);
+     GFunctor (excl_authR stenning_A_stateO);
+     GFunctor (excl_authR stenning_B_stateO) ].
+
+Global Instance subG_stenningΣ {Σ} : subG stenningΣ Σ → stenningPreG Σ.
+Proof. solve_inG. Qed.
+
+Section with_Σ.
+  Context `{anerisG _ _ (live_model_of_user stenning_model) Σ}.
+  Context `{!stenningG Σ}.
+  Let Ns := nroot .@ "stenning".
+
+  Definition retinv : iProp Σ := frag_free_roles_are ∅ ∗
+    ∃ stA stB, frag_model_is (stA, stB) ∗ own stenning_A_name (●E stA) ∗ own stenning_B_name (●E stB).
+
+  Lemma token_update γ {A: ofe} {_: inG Σ (excl_authR A)} (st st' st'' : A) :
+    own γ (●E st) ∗ own γ (◯E st'') ==∗ own γ (●E st') ∗ own γ (◯E st').
+  Proof.
+    rewrite -!own_op. iApply own_update. apply excl_auth_update.
+  Qed.
+
+                                               (*  TODO:   can we do better?     *)
+  Lemma token_agree γ {A: ofe} `{OfeDiscrete A, @LeibnizEquiv A (ofe_equiv A)} {_: inG Σ (excl_authR A)} (st st' : A) :
+    own γ (●E st) -∗ own γ (◯E st') -∗ ⌜ st = st' ⌝.
+  Proof.
+    iIntros "HA HB". iCombine "HB HA" as "H".
+    iDestruct (own_valid with "H") as "%Hval".
+    iPureIntro. by apply excl_auth_agree_L.
+  Qed.
+
+  Definition ipA := ip_of_address saA.
+  Definition ipB := ip_of_address saB.
+
+  Lemma wp_client tid (f : nat) (Hf: f > 40) :
+    {{{ inv Ns retinv ∗ is_node ipA ∗ saA ⤇ (λ msg, ⌜ msg = msg⌝) ∗ saB ⤇ (λ msg, ⌜ msg = msg⌝) ∗
+          own stenning_A_name (◯E (AReceiving 0)) ∗
+          (ipA, tid) ↦M {[ Arole := f ]} ∗ saA ⤳ (∅, ∅) ∗
+          free_ports (ip_of_address saA) {[port_of_address saA]} }}}
+      (mkExpr (ip_of_address saA) (client saA saB #())) @ (ipA, tid); ⊤
+    {{{ v, RET v; (ipA, tid) ↦M ∅ }}}.
+  Proof.
+    iIntros (Φ) "(Hinv&#Hin&HsA&HsB&Hst&Hf&HRT&Hfp) HΦ".
+    rewrite /client.
+    wp_pure _.
+
+    wp_bind (NewSocket _).
+    iApply sswp_MU_wp. iApply wp_new_socket=>//.
+    iIntros (sh) "Hsh".
+    mu_fuel.
+
+    iApply wp_value'. do 2 wp_pure _.
+
+    wp_bind (SocketBind _ _).
+    iApply sswp_MU_wp. iApply (wp_socketbind with "[Hfp] [Hsh]") =>//=; first done.
+    iIntros "Hsh".
+    mu_fuel.
+    iApply wp_value'.
+    do 2 wp_pure _.
+
+    wp_bind (SetReceiveTimeout _ _ _).
+    iApply sswp_MU_wp. iApply (wp_rcvtimeo_ublock NotStuck ⊤ (ipA, tid) sh _ saA 1 1 with "[Hsh]").
+    3: { auto. }
+    { done. }
+    { lia. }
+    iIntros "Hsh". mu_fuel. iApply wp_value'. do 5 wp_pure _.
+
+    iAssert (∃ (f : nat), ⌜ f > 25 ⌝ ∗ (ipA, tid) ↦M <[Arole:=f]> ∅)%I
+      with "[Hf]" as (f') "[Hf' Hf]".
+    { iExists _. iFrame. iPureIntro. lia. }
+    clear f Hf.
+
+    iAssert (∃ R T, saA ⤳ (R, T))%I with "[HRT]" as (R T) "HRT".
+    { iExists _, _. iFrame. }
+
+    (* TODO: generalize 0 *)
+    iLöb as "IH" forall (f' R T) "Hf".
+  Admitted.
+
+  Lemma wp_sever tid (f : nat) (Hf: f > 40) :
+    {{{ inv Ns retinv ∗ is_node ipA ∗ saA ⤇ (λ msg, ⌜ msg = msg⌝) ∗ saB ⤇ (λ msg, ⌜ msg = msg⌝) ∗
+          own stenning_B_name (◯E (BReceiving 0)) ∗
+          (ipB, tid) ↦M {[ Brole := f ]} ∗ saB ⤳ (∅, ∅) ∗
+          free_ports (ip_of_address saA) {[port_of_address saA]} }}}
+      (mkExpr (ip_of_address saA) (server saA saB)) @ (ipA, tid); ⊤
+    {{{ v, RET v; (ipA, tid) ↦M ∅ }}}.
+  Proof.
+  Admitted.
+
+End with_Σ.
